Put kruskal and UF specs into one file so that I can make a joint Gprog for them to use. Now VST can "see" UF's methods when verifying body_kruskal.

kruskal/verif_kruskal_edgelist.v
@@ -21,106 +21,13 @@ Require Import RamifyCoq.kruskal.spatial_wedgearray_graph.
 Require Import RamifyCoq.sample_mark.spatial_array_graph.
 (*spanning tree definition*)
 Require Import RamifyCoq.kruskal.mst.
+Require Import RamifyCoq.kruskal.kruskal_uf_specs.
 (*Require Import RamifyCoq.graph.spanning_tree.*)
 
 Local Open Scope Z_scope.
 
 (*I guess we ought to throw these in a specs_kruskal.v
 Also, thinking of we can combine env and spatial*)
-
-(*Taken from VST's queue*)
-Definition mallocK_spec :=
- DECLARE _mallocK
-  WITH sh: wshare, n: Z
-  PRE [tint]
-     PROP (4 <= n <= Int.max_unsigned)
-     PARAMS (Vint (Int.repr n))
-     GLOBALS ()
-     SEP ()
-  POST [ tptr tvoid ]
-     EX v: pointer_val,
-     PROP (malloc_compatible n (pointer_val_val v))
-     LOCAL (temp ret_temp (pointer_val_val v))
-     SEP (memory_block sh n (pointer_val_val v)).
-
-(*It'll be useful if we can come up with some freeN spec, then centralize these in some header*)
-
-Definition init_empty_graph_spec :=
-  DECLARE _init_empty_graph
-  WITH gv: globals, sh: wshare
-  PRE []
-     PROP ()
-     PARAMS ()
-     GLOBALS (gv)
-     SEP (data_at sh tint (Vint (Int.repr MAX_EDGES)) (gv _MAX_EDGES))
-  POST [ tptr t_wedgearray_graph ]
-     EX gptr eptr: pointer_val,
-     PROP ()
-     LOCAL (temp ret_temp (pointer_val_val gptr))
-     SEP (data_at sh tint (Vint (Int.repr MAX_EDGES)) (gv _MAX_EDGES) *
-          wedgearray_graph_rep sh empty_FiniteWEdgeListGraph gptr eptr).
-
-(*
-This is the modified sort spec from cbench. It's rather ugly imo
-
-wedgerep := reptype t_struct_edge
-Definitions like sorted and wedge_le are thrown into env_kruskal
-
-The call should look something like:
-forward_call (sh, pointer_val_val orig_eptr, 0, numE g, nil, map wedge_to_cdata ... , nil).
-
-The result PROPs (Permutation al bl; sorted wedge_le bl) have to be massaged to imply
-  the first edge (w,u,v) encountered in kruskal's loop has lower w than other (_,u,v)s after it
-*)
-Definition sort_edges_spec :=
- DECLARE _sort_edges
-  WITH sh: share, a: val, m: int, n: int, before: list wedgerep, al: list wedgerep, after: list wedgerep
-  PRE  [tptr t_struct_edge, tint, tint] 
-    PROP( readable_share sh; writable_share sh;
-          Int.min_signed <= Zlength (before++al++after) <= Int.max_signed;
-          if zlt (Int.signed m) (Int.signed n)
-            then   (Zlength before = Int.signed m 
-                     /\ Zlength after = (Zlength (before++al++after))-(Int.signed n+1)
-                     /\ Zlength al = Int.signed n+1- Int.signed m)
-            else al=nil;
-            Forall def_wedgerep al)
-    PARAMS(a; Vint m; Vint n) GLOBALS ()
-    SEP(data_at sh (tarray t_struct_edge (Zlength (before++al++after)))
-             (before ++ al ++ after) a)
-  POST [ tvoid ]
-    EX bl: list wedgerep,
-     PROP(Permutation al bl; sorted wedge_le bl) 
-     LOCAL ()
-    SEP(data_at sh (tarray t_struct_edge (Zlength (before++al++after)))
-             (before ++ bl ++ after) a).
-
-Definition kruskal_spec :=
-  DECLARE _kruskal
-  WITH gv: globals, sh: wshare, g: FiniteWEdgeListGraph, orig_gptr : pointer_val, orig_eptr : pointer_val
-  PRE [tptr t_wedgearray_graph]
-   PROP (sound_weighted_edge_graph g; numE g <= MAX_EDGES
-        )
-   PARAMS ((pointer_val_val orig_gptr))
-   GLOBALS (gv)
-   SEP (data_at sh tint (Vint (Int.repr MAX_EDGES)) (gv _MAX_EDGES);
-        wedgearray_graph_rep sh g orig_gptr orig_eptr)
-  POST [tptr t_wedgearray_graph]
-   EX msf_gptr msf_eptr: pointer_val,
-   EX (msf: FiniteWEdgeListGraph),
-   PROP (sound_weighted_edge_graph msf;
-        (numE msf) <= MAX_EDGES;
-        minimum_spanning_forest (lg_gg g) (lg_gg msf)
-                                 Z.add
-                                 0
-                                 Z.le)
-   LOCAL (temp ret_temp (pointer_val_val msf_gptr))
-   SEP (data_at sh tint (Vint (Int.repr MAX_EDGES)) (gv _MAX_EDGES);
-        wedgearray_graph_rep sh g orig_gptr orig_eptr;
-       wedgearray_graph_rep sh msf msf_gptr msf_eptr).
-
-Definition Vprog : varspecs. mk_varspecs prog. Defined.
-Definition Gprog : funspecs := ltac:(with_library prog
-  [mallocK_spec; init_empty_graph_spec; kruskal_spec]).
 
 Lemma body_init_empty_graph: semax_body Vprog Gprog f_init_empty_graph init_empty_graph_spec.
 Proof.
@@ -162,6 +69,15 @@ rewrite empty_WEdgeListGraph_numV. rewrite empty_WEdgeListGraph_numE.
 simpl. rewrite data_at_zero_array_eq. entailer!.
 reflexivity. apply H4. rewrite empty_WEdgeListGraph_graph_to_wedgelist. simpl. reflexivity.
 Qed.
+
+Lemma body_kruskal: semax_body Vprog Gprog f_kruskal kruskal_spec.
+Proof.
+  start_function.
+  unfold wedgearray_graph_rep. Intros.
+  forward. forward.
+  Fail forward_call.
+
+Abort.
 
 
 
